sha3/proof/TopLevel.ec
@@ -1,25 +1,9 @@
 (* -------------------------------------------------------------------- *)
 require import Pair Int Real List.
 require (*--*) IRO LazyRP Indifferentiability.
-(*---*) import Dprod.
 
 (* -------------------------------------------------------------------- *)
-(* Replay Common.ec *)
-op r : { int | 0 < r } as gt0_r.
-op c : { int | 0 < c } as gt0_c.
-
-type block.
-type capacity.
-
-op cdist : capacity distr.
-op bdist : block distr.
-
-op b0 : block.
-op c0 : capacity.
-
-op b2bits : block -> bool list.
-
-op (^) : block -> block -> block.
+require import Common.
 
 (* -------------------------------------------------------------------- *)
 op pad : bool list -> block list.
@@ -29,12 +13,6 @@ clone import IRO as BIRO with
   type from <- bool list,
   type to <- bool,
   op valid (x : bool list) <- true.
-
-clone import LazyRP as Perm with
-  type D <- block * capacity,
-  op   d <- bdist * cdist
-
-  rename [module] "P" as "Perm".
   
 (* -------------------------------------------------------------------- *)
 clone include Indifferentiability.Core with
@@ -49,12 +27,12 @@ import Types.
 
 (* -------------------------------------------------------------------- *)
 (** Spurious uninitialized variable warning on p *)
-module Sponge (P : RP) : BIRO.IRO, CONSTRUCTION(P) = {
+module Sponge (P : PRIMITIVE) : BIRO.IRO, CONSTRUCTION(P) = {
   proc init = P.init
 
   proc f(bp : bool list, n : int): bool list = {
     var z       <- [];
-    var (sa,sc) <- (b0, c0);
+    var (sa,sc) <- (b0, Capacity.c0);
     var i       <- 0;
     var p       <- pad bp;
 
@@ -65,7 +43,7 @@ module Sponge (P : RP) : BIRO.IRO, CONSTRUCTION(P) = {
     }
     (* Squeezing *)
     while (i < (n + r - 1) /% r) {
-      z       <- z ++ (b2bits sa);
+      z       <- z ++ (Block.w2bits sa);
       (sa,sc) <@ P.f(sa,sc);
     }
 
