sha3/proof/BlocksToTopLevel.ec
@@ -1,0 +1,82 @@
+(* -------------------------------------------------------------------- *)
+require import Fun Pred Option Pair Int Real List FSet NewFMap.
+require (*--*) Blocks TopLevel.
+
+(* -------------------------------------------------------------------- *)
+require import Common.
+print Common.
+
+op chunk: bool list -> bool list list.
+
+op padlength (n : int) =
+  let n' = (n + 2) %% r in
+  if n' = 0 then 0 else r - n'.
+
+op pad (bs : bool list): block list =
+  let p = rcons (true :: mkseq (fun k => false) (padlength (size bs))) true in
+  map bits2w (chunk (bs ++ p)).
+
+op unpad (bs : block list): bool list option. (* Alley to fill in the definition *)
+
+axiom unpadK (bs : bool list): pcancel pad unpad.
+axiom padK (*?*) (bs : block list): ocancel unpad pad.
+
+op valid_lower (bs : block list) = unpad bs <> None.
+
+clone Blocks as Lower with
+  op valid <- valid_lower.
+
+clone TopLevel as Upper.
+
+(* -------------------------------------------------------------------- *)
+module UpperFun ( F : Lower.FUNCTIONALITY ) = {
+  proc init = F.init
+
+  proc f(p : bool list, n : int) = {
+    var bs;
+
+    bs  <@ F.f(pad p,(n + r - 1) /% r);
+    return take n (flatten (map w2bits bs));
+  }
+}.
+
+module LowerFun ( F: Upper.FUNCTIONALITY) = {
+  proc init = F.init
+
+  proc f(p : block list, n : int) = {
+    var bs, m;
+    var bs' <- [];
+
+    m <- unpad p;
+    if (m <> None) {
+      bs  <@ F.f(oget m,n * r);
+      bs' <- map bits2w (chunk bs);
+    }
+    return bs';
+  }
+}.
+
+(* -------------------------------------------------------------------- *)
+equiv ModularConstruction:
+  UpperFun(Lower.BlockSponge(Perm)).f ~ Upper.Sponge(Perm).f:
+    ={glob Perm, arg} ==> ={glob Perm, res}.
+proof.
+  proc. inline Lower.BlockSponge(Perm).f.
+  admit. (* done *)
+qed.
+
+module ModularSimulator (S : Lower.SIMULATOR, F : Upper.FUNCTIONALITY) = S(LowerFun(F)).
+
+module LowerDist ( D : Upper.DISTINGUISHER, F : Lower.FUNCTIONALITY, P : PRIMITIVE) =
+  D(UpperFun(F),P).
+
+section.
+  declare module LowerSim : Lower.SIMULATOR.
+  declare module UpperDist : Upper.DISTINGUISHER.
+
+  lemma Conclusion &m:
+    `|Pr[Upper.RealIndif(Upper.Sponge,Perm,UpperDist).main() @ &m: res]
+      - Pr[Upper.IdealIndif(Upper.BIRO.IRO',ModularSimulator(LowerSim),UpperDist).main() @ &m: res]|
+    = `|Pr[Lower.RealIndif(Lower.BlockSponge,Perm,LowerDist(UpperDist)).main() @ &m: res]
+      - Pr[Lower.IdealIndif(Lower.BIRO.IRO',LowerSim,LowerDist(UpperDist)).main() @ &m: res]|.
+  proof. admit. qed.
